theories/SemSound.v
@@ -37,45 +37,47 @@ Proof.
     unfold PropOnItem.
 Admitted.
 
+
 Theorem soundout : forall G e e' s eta p,
     Typed G e s ->
-    Step eta e e' p ->
-    WFTerm (fv G) e ->
+    (* WFTerm (fv G) e -> *)
     WFContext G ->
     EnvTyped eta G ->
+    Step eta e e' p ->
     PfxTyped p s
 .
 Proof.
-    intros G e e' s eta p Hty.
+    intros G e e' s eta p Hty HwfG.
     generalize dependent e'.
     generalize dependent eta.
     generalize dependent p.
-    induction Hty; intros p eta e0' Hstep Hwfe HwfG Heta.
-    - sinvert Hwfe. cbn in *. sauto q: on.
-    - sinvert Hwfe; sinvert Hstep.
-      assert (~fv G x) by sfirstorder use:fv_fill.
-      assert (~fv G y) by sfirstorder use:fv_fill.
-      assert (PfxTyped (PfxParPair p1 p2) (Types.TyPar s t)) by qauto l:on use: maps_to_has_type.
-      sinvert H1.
-      eapply IHHty.
-      + eauto.
-      + eapply wf_iff; [| eauto]. intro. admit. (* i think we can do this. *)
-      + apply wf_fill in HwfG. destruct HwfG as [A [B C]].
-        apply wf_fill.
-        (* here, we need to know that x and y are not free in G.*)
-        split; try split. sfirstorder. sauto l: on. cbn in *. sfirstorder use:fv_fill.
-      + eapply fill_replace; [|eauto| |]. admit.
-        * eapply env_typed_comma; [| eapply env_typed_singleton; eauto | eapply env_typed_singleton; eauto]. admit.
-        * admit.
-    - sinvert Hwfe; sinvert HwfG; sinvert Heta. sinvert Hstep; admit.
-    - sinvert Hwfe. admit.
-    - sinvert Hwfe. admit.
-    - sinvert Hwfe. admit.
-    - sinvert Hwfe. apply wf_fill in HwfG.
-      destruct HwfG as [U []]. sinvert H. apply fv_fill in H1.
+    induction Hty; intros p eta e0' Heta Hstep.
+    - cbn in *. sauto q: on.
+    - sinvert Hstep.
+      assert (~fv G z) by hauto q: on use:wf_fill.
+      eapply IHHty; [| | eauto].
+      + qauto l: on use: hmm'.
+      + eapply catlenvtyped; eauto; sauto l: on use: maps_to_has_type.
+    - sinvert HwfG; sinvert Heta. sinvert Hstep.
+      + constructor. eapply IHHty1; eauto.
+      + constructor. eapply IHHty1; eauto. eauto. eauto.
+    - sinvert Hstep; eapply IHHty; [| | eauto | | | eauto].
+      + eapply hmm'; eauto.
+      + eapply catrenvtyped1; eauto. sauto l: on use: maps_to_has_type.
+      + eapply hmm'; eauto.
+      + assert (PfxTyped (PfxCatBoth p1 p2) (Types.TyDot s t)) by sauto l: on use: maps_to_has_type.
+        sinvert H2.
+        eapply catrenvtyped2; eauto. 
+    - sauto lq: on.
+    - sauto lq: on.
+    - sinvert Hstep. 
       sauto use: maps_to_has_type.
     - sfirstorder.
-    - sinvert Hstep.
+    - sinvert Hstep. eapply IHHty2; [ | | eauto].
+      + sauto l: on use:wf_fill.
+      + eapply letenvtyped; [| eauto].
+        eapply IHHty1; [| | eauto]. sfirstorder use:wf_fill. sfirstorder use:maps_to_hole.
+    - sinvert Hstep. eapply IHHty; [ | | eauto]. hauto lq: on rew: off use: wf_fill.
 Admitted.
 
 (*
