theories/SinkTm.v
@@ -1,0 +1,10 @@
+From LambdaST Require Import
+  Ident
+  Types
+  Terms
+  Prefix.
+From Hammer Require Import
+  Tactics.
+
+(* TODO: fix with definintion. *)
+Fixpoint sinkTm (p : prefix) : term := TmSink.
