theories/Typing.v
@@ -19,6 +19,9 @@ Inductive Typed : context -> term -> type -> Prop :=
       G |- e2 \in t ->
       G |- (TmComma e1 e2) \in (TyPar s t)
   | T_Par_L : forall G x y z s t e r,
+      x <> y ->
+      ~fv G x ->
+      ~fv G y ->
       fill G (CtxComma (CtxHasTy x s) (CtxHasTy y t)) |- e \in r ->
       fill G (CtxHasTy z (TyPar s t)) |- (TmLetPar x y z e) \in r
   | T_Cat_R : forall G D e1 e2 s t,
@@ -26,8 +29,11 @@ Inductive Typed : context -> term -> type -> Prop :=
       D |- e2 \in t ->
       (CtxSemic G D) |- (e1; e2) \in (TyDot s t)
   | T_Cat_L : forall G x y z s t e r,
+      x <> y ->
+      ~fv G x ->
+      ~fv G y ->
       fill G (CtxSemic (CtxHasTy x s) (CtxHasTy y t)) |- e \in r ->
-      fill G (CtxHasTy z (TyPar s t)) |- (TmLetCat t x y z e) \in r
+      fill G (CtxHasTy z (TyDot s t)) |- (TmLetCat t x y z e) \in r
   | T_Eps_R : forall G,
       G |- sink \in eps
   | T_One_R : forall G,
@@ -39,9 +45,13 @@ Inductive Typed : context -> term -> type -> Prop :=
       G' |- e \in s ->
       G |- e \in s
   | T_Let : forall G D x e e' s t,
+      ~(fv G x) ->
       D |- e \in s ->
       fill G (CtxHasTy x s) |- e' \in t ->
       fill G D |- TmLet x e e' \in t
+  | T_Drop : forall G x s t e,
+      fill G CtxEmpty |- e \in t ->
+      fill G (CtxHasTy x s) |- TmDrop x e \in t
 where "G '|-' x '\in' T" := (Typed G x T).
 Hint Constructors Typed : core.
 
@@ -62,5 +72,6 @@ Proof.
     - sfirstorder use: fv_fill.
     - sfirstorder.
     - destruct Hfv; hauto q: on use: fv_fill.
+    - hauto q: on use:fv_fill.
 Qed.
 Hint Resolve typing_fv : core.
